update library for delete proof

concurrency/bst_template_lib.v
@@ -1257,3 +1257,605 @@ Proof.
       * apply prop_right. now apply riit_root.
       * cancel. rewrite <- wand_sepcon_adjoint. cancel.
 Qed.
+
+(*support delete*)
+
+Ltac allpr_intros x := apply allp_right; intros x. (* Temporary *)
+
+Lemma gt_ghost_sorted : forall t1 t2 k k0 v0 g g0,
+  gt_ghost (T_ghost t1 g k0 v0 t2 g0) k ->
+  gt_ghost (V := val) t1 k /\ gt_ghost (V := val) t2 k.
+Proof.
+  intros. unfold gt_ghost in H.
+  split; unfold gt_ghost; intros; apply H.
+  * apply InLeft_ghost; auto.
+  * apply InRight_ghost; auto.
+Qed.
+
+Ltac logic_to_iris :=
+  match goal with |-context[(|==> ?P)%logic] => change ((|==> P)%logic) with ((|==> P)%I) end.
+
+Lemma change_ghost_root: forall tg gl rootl rootr,
+  sorted_ghost_tree tg ->
+  ghost_tree_rep tg gl (rootl, rootr) |--
+  EX o : option ghost_info,
+    !! (match o with
+        | None => tg = E_ghost
+        | Some (x, y, g1, g2) => (exists tg1 tg2, tg = T_ghost tg1 g1 x y tg2 g2)
+        end) &&
+    (public_half gl (rootl, rootr, Some o)) *
+    (ALL rootl2 : number, ALL rootr2 : number, ALL g : gname,
+      !! (range_incl (rootl, rootr) (rootl2, rootr2) = true) &&
+      public_half g (rootl2, rootr2, Some o) -* |==> ghost_tree_rep tg g (rootl2, rootr2)).
+Proof.
+  induction tg; intros.
+  - simpl. Exists (None: @option ghost_info). entailer!.
+    allpr_intros rootl2; allpr_intros rootr2; allpr_intros g.
+    rewrite <- wand_sepcon_adjoint. rewrite emp_sepcon. Intros.
+    apply ghost_seplog.bupd_intro.
+  - simpl. Exists (Some (k, v, g, g0)). entailer!. { eauto. }
+    allpr_intros rootl2; allpr_intros rootr2; allpr_intros g'.
+    inv H. sep_apply IHtg1. sep_apply IHtg2.
+    Intros o1 o2.
+    rewrite <- wand_sepcon_adjoint.
+    iIntros "((Ha & Hb) & Hc)". logic_to_iris.
+    iDestruct "Ha" as "[root_left tree_left]".
+    iDestruct "Hb" as "[root_right tree_right]".
+    iSpecialize ("tree_left" $! (Finite_Integer k) rootr2  g0).
+    iSpecialize ("tree_right" $! rootl2 (Finite_Integer k) g).
+    iDestruct "Hc" as "[% Hc]". apply andb_prop in H1. destruct H1.
+    assert (range_incl (rootl, Finite_Integer k) (rootl2, Finite_Integer k) = true).
+    {
+      apply andb_true_intro. split; try apply less_than_equal_refl. auto.
+    }
+    assert (range_incl (Finite_Integer k, rootr) (Finite_Integer k, rootr2) = true).
+    {
+      apply andb_true_intro. split; try apply less_than_equal_refl. auto.
+    }
+    iMod (public_half_range_incl with "root_right") as "root_right".
+    { eauto. }
+    iMod (public_half_range_incl with "root_left") as "root_left".
+    { eauto. }
+    repeat logic_to_iris.
+    iMod ("tree_right" with "[$root_right]"). iPureIntro.
+    split; auto.
+    iMod ("tree_left" with "[$root_left]"). iPureIntro.
+    split; auto. iModIntro. iFrame.
+Qed.
+
+Fixpoint pushdown_ghost {V} (c ab: @ghost_tree V) : ghost_tree :=
+  match ab with
+  | E_ghost => c
+  | T_ghost a ga y v' b gb => T_ghost (pushdown_ghost c a) ga y v' b gb
+  end.
+
+  Fixpoint delete_ghost {V} (x: key) (s: @ghost_tree V) : ghost_tree :=
+    match s with
+    | E_ghost => E_ghost
+    | T_ghost a ga y v' b gb => if  (Z.ltb x y) then T_ghost (delete_ghost x a) ga y v' b gb
+                                else if  (Z.ltb y x) then T_ghost a ga y v' (delete_ghost x b) gb
+                                else pushdown_ghost a b
+    end.
+
+Arguments range_incl : simpl never.
+
+(* up *)
+Lemma Subtract_Union1 : forall {A} S1 S2 (x : A),
+    ~Ensembles.In S2 x ->
+    Subtract (Union S1 S2) x = Union (Subtract S1 x) S2.
+Proof.
+  intros; apply Extensionality_Ensembles; split; intros ? Hin.
+  - inv Hin.
+    inv H0.
+    + constructor 1; constructor 1; auto.
+    + constructor 2; auto.
+  - inv Hin.
+    + inv H0.
+      constructor; auto.
+      constructor 1; auto.
+    + constructor.
+      constructor 2; auto.
+      { intros X; inv X; contradiction. }
+Qed.
+
+Lemma Subtract_Add : forall {A} S (x : A), ~Ensembles.In S x -> Subtract (Add S x) x = S.
+Proof.
+  intros; apply Extensionality_Ensembles; split; intros ??.
+  - inv H0.
+    inv H1; auto; contradiction.
+  - constructor.
+    + constructor 1; auto.
+    + intros X; inv X; contradiction.
+Qed.
+
+Lemma In_same_map : forall tg1 tg2 x, tree_to_gmap tg1 = tree_to_gmap tg2 -> In_ghost x tg1 <-> In_ghost x tg2.
+Proof.
+  intros.
+  rewrite !In_tree_to_gmap H; reflexivity.
+Qed.
+
+Lemma ghost_tree_delete: forall tg g_root g_in gl gr x v (r_root: range),
+ Ensembles.In (find_ghost_set tg g_root) g_in ->
+ keys_in_range_ghost tg r_root ->
+ sorted_ghost_tree tg -> unique_gname tg ->
+ ~Ensembles.In (find_ghost_set' tg) g_root ->
+ ghost_tree_rep tg g_root r_root |--
+ EX n n0:number, EX o1:option ghost_info,
+ !!(range_incl (n,n0) r_root = true) &&
+ public_half g_in (n, n0, Some o1) *
+ (!!(o1 = Some (x,v,gl,gr)) -->
+   EX o3 : option ghost_info,
+  public_half gr (Finite_Integer x, n0, Some o3) *
+ ((EX o2 : option ghost_info,
+        public_half gl (n, Finite_Integer x, Some o2) * 
+   (!!(o1 = Some (x,v,gl,gr) /\ o3 = None /\ (key_in_range x (n,n0) = true)) &&
+      public_half g_in (n, n0, Some (* o1' *) o2) -* |==> (!! (In_ghost x tg
+        /\ find_ghost_set (delete_ghost x tg) g_root = (Subtract (Subtract (find_ghost_set tg g_root) gl) gr)
+        /\ Ensembles.In (find_ghost_set' tg) gl /\ Ensembles.In (find_ghost_set' tg) gr)
+        && ghost_tree_rep (delete_ghost x tg) g_root r_root))%I)
+
+   && (ALL gr1 gr2 : gname, ALL k : key, ALL y : val,
+        (!!(o1 = Some (x,v,gl,gr) /\ o3 = Some (k, y, gr1, gr2)
+          /\ (key_in_range x (n,n0) = true) /\ less_than (Finite_Integer x) (Finite_Integer k) = true) &&
+        (public_half g_in (n, n0, Some (Some (k, y, gr, gr2)))
+        * public_half gr (n, Finite_Integer k, Some (Some (x, v, gl, gr1))))
+        -* |==> (EX tg',
+          !!(tree_to_gmap tg = tree_to_gmap tg' /\
+             find_ghost_set' tg = find_ghost_set' tg' /\
+             sorted_ghost_tree tg' /\ unique_gname tg') &&
+           ghost_tree_rep tg' g_root r_root)))%I)).
+Proof.
+  induction tg; destruct r_root as (rootl, rootr); simpl; intros Hin Hrange Hsorted Hunique Hroot.
+  - inv Hin.
+    Exists rootl rootr (None : @option ghost_info).
+    rewrite range_incl_refl; entailer!.
+    rewrite <- imp_andp_adjoint. Intros; discriminate.
+  - apply keys_in_range_ghost_subtrees in Hrange as (Hk & Hl & Hr); auto.
+    inv Hsorted; inv Hunique; inv Hin. inv H.
+    + eapply IHtg1 in H0; [| eauto | eauto | eauto | eauto].
+      simpl in H0; sep_apply H0; clear H0.
+      Intros n1 n2 o1; Exists n1 n2 o1; entailer!.
+      { eapply range_incl_trans; [eauto|].
+        apply (key_in_range_l _ (_, _)); auto. }
+      rewrite <- imp_andp_adjoint. Intros; subst.
+      rewrite -> prop_imp by reflexivity.
+      Intros o3 o2; Exists o3 o2; cancel.
+      iIntros "((Hcase & ?) & ?)"; iSplit.
+      * iDestruct "Hcase" as "[[$ IH] _]".
+        iIntros "[(% & % & %) Hin]"; subst.
+        iMod ("IH" with "[$Hin]") as "[(% & % & % & %) Hdel]"; [auto|].
+        specialize (Hgtl _ H1).
+        destruct (Z.ltb x k) eqn:?; [simpl; iFrame | lia].
+        iPureIntro; split; auto; split3.
+        -- apply InLeft_ghost; auto.
+        -- rewrite -> empty_intersection in H8.
+            rewrite H3 !Subtract_Union1; auto.
+            ** rewrite find_ghost_set_equiv; intros X; inv X.
+               unshelve eapply (H8 _ _ H14); eauto.
+               inv H14; contradiction.
+            ** rewrite find_ghost_set_equiv; intros X; inv X.
+               unshelve eapply (H8 _ _ H14); eauto.
+               inv H14; contradiction.
+            ** intros X; inv X.
+               contradiction Hroot; constructor 1.
+               rewrite find_ghost_set_equiv; constructor 1; auto.
+            ** intros X; inv X.
+               contradiction Hroot; constructor 1.
+               rewrite find_ghost_set_equiv; constructor 1; auto.
+        -- split; rewrite find_ghost_set_equiv; do 2 constructor 1; auto.
+      * iIntros (gr1 gr2 k0 y) "[(% & % & % & %) H]".
+        iDestruct "Hcase" as "[_ IH]".
+        logic_to_iris.
+        iMod ("IH" $! gr1 gr2 k0 y with "[$H]") as (tg') "[(% & % & % & %) IH]"; [auto | subst].
+        iExists (T_ghost tg' g k v tg2 g0); simpl; iFrame.
+        iPureIntro; split; auto; split3.
+        -- congruence.
+        -- rewrite !find_ghost_set_equiv; congruence.
+        -- split; constructor; rewrite <- ?H13; auto.
+           intros ??; eapply Hgtl, In_same_map; eassumption.
+    + eapply IHtg2 in H0; [| eauto | eauto | eauto | eauto].
+      simpl in H0; sep_apply H0; clear H0.
+      Intros n1 n2 o1; Exists n1 n2 o1; entailer!.
+      { eapply range_incl_trans; [eauto|].
+        apply (key_in_range_r _ (_, _)); auto. }
+      rewrite <- imp_andp_adjoint; Intros; subst.
+      rewrite -> prop_imp by reflexivity.
+      Intros o3 o2; Exists o3 o2; cancel.
+      iIntros "((Hcase & ?) & ?)"; iSplit.
+      * iDestruct "Hcase" as "[[$ IH] _]".
+        iIntros "[(% & % & %) Hin]"; subst.
+        iMod ("IH" with "[$Hin]") as "[(% & % & % & %) Hdel]"; [auto|].
+        specialize (Hltr _ H1).
+        destruct (Z.ltb x k) eqn:?; [lia|].
+        destruct (Z.ltb k x) eqn:?; [simpl; iFrame | lia].
+        iPureIntro; split; auto; split3.
+        -- apply InRight_ghost; auto.
+        -- rewrite -> empty_intersection in H8.
+            rewrite H3 Subtract_Union1.
+            rewrite Subtract_Union1.
+            rewrite (invariants.Union_comm _ (find_ghost_set _ _)) !Subtract_Union1.
+            rewrite (invariants.Union_comm _ (find_ghost_set _ _)); auto.
+            ** rewrite find_ghost_set_equiv; intros X; inv X.
+               eapply (H8 _ H14); eauto.
+               inv H14; contradiction.
+            ** rewrite find_ghost_set_equiv; intros X; inv X.
+               eapply (H8 _ H14); eauto.
+               inv H14; contradiction.
+            ** intros X; inv X.
+               contradiction Hroot; constructor 2.
+               rewrite find_ghost_set_equiv; constructor 1; auto.
+            ** intros X; inv X.
+               contradiction Hroot; constructor 2.
+               rewrite find_ghost_set_equiv; constructor 1; auto.
+        -- split; rewrite !find_ghost_set_equiv; constructor 2; constructor 1; auto.
+      * iIntros (gr1 gr2 k0 y) "[(% & % & % & %) H]".
+        iDestruct "Hcase" as "[_ IH]".
+        logic_to_iris.
+        iMod ("IH" $! gr1 gr2 k0 y with "[$H]") as (tg') "[(% & % & % & %) IH]"; [auto | subst].
+        iExists (T_ghost tg1 g k v tg' g0); simpl; iFrame.
+        iPureIntro; split; auto; split3.
+        -- congruence.
+        -- rewrite !find_ghost_set_equiv; congruence.
+        -- split; constructor; rewrite <- ?H13; auto.
+           intros ??; eapply Hltr, In_same_map; eassumption.
+    + clear IHtg1 IHtg2. inv H. (* pushdown case *)
+      Exists rootl rootr (Some (k, v, g, g0)); rewrite range_incl_refl; entailer!.
+      rewrite <- imp_andp_adjoint; Intros. inv H.
+      erewrite change_ghost_root by auto; Intros o2.
+      destruct tg2; simpl.
+      * Exists (None : @option ghost_info); cancel. apply andp_right.
+        Exists o2; cancel. rewrite Z.ltb_irrefl. rewrite <- wand_sepcon_adjoint. entailer!.
+        iIntros "(Ha & Hb)". iSpecialize ("Ha" $! rootl rootr g_in with "[$Hb]").
+        { iPureIntro; split; auto. apply (key_in_range_l _ (_, _)); auto. }
+        logic_to_iris. iMod "Ha" as "$"; iPureIntro.
+        split; auto; split3.
+        -- constructor 1; auto.
+        -- unfold Add; rewrite -> 3Subtract_Union1, (find_ghost_set_equiv _ gl).
+            fold (Add (find_ghost_set tg1 gl) gr). rewrite -> Subtract_Add by auto.
+            fold (Add (find_ghost_set' tg1) gr). rewrite -> Subtract_Add by auto.
+            apply find_ghost_set_equiv.
+            { intros X; inv X; contradiction. }
+            { intros X; inv X. contradiction Hroot. constructor 2; rewrite find_ghost_set_equiv; constructor 2; constructor. }
+            { intros X; inv X. contradiction Hroot. constructor 1; rewrite find_ghost_set_equiv; constructor 2; constructor. }
+        -- split; [constructor 1; rewrite find_ghost_set_equiv|]; constructor 2; constructor.
+        -- allpr_intros gr1; allpr_intros gr2; allpr_intros k; allpr_intros y.
+           rewrite <- wand_sepcon_adjoint; Intros; discriminate.
+      * Exists (Some (k, v, g, g0)) o2; cancel. apply andp_right.
+        { cancel. rewrite <- wand_sepcon_adjoint; Intros; discriminate. }
+        allpr_intros gr1; allpr_intros gr2; allpr_intros k'; allpr_intros y.
+        rewrite <- wand_sepcon_adjoint; entailer!.
+        iIntros "(((((Ha & Hb) & Hc) & Hd) & He) & Hf)".
+        iSpecialize ("Hb" $! rootl (Finite_Integer x) gl with "[$Ha]").
+        { rewrite range_incl_refl; auto. }
+        inv H0. logic_to_iris. iMod "Hb"; iModIntro.
+        iExists (T_ghost (T_ghost tg1 gl x v0 tg2_1 gr1) gr k' y tg2_2 gr2); simpl; iFrame.
+        iPureIntro; split; auto; split3; [.. | split].
+        -- rewrite <- insert_union_l, <- insert_union_r, insert_commute, map_union_assoc; auto.
+           { lia. }
+           { destruct (eq_dec (tree_to_gmap tg1 !! k') None); auto. apply In_tree_to_gmap in n. specialize (Hgtl _ n); lia. }
+        -- unfold Add; rewrite !invariants.Union_assoc.
+           rewrite (invariants.Union_comm (Singleton _)); auto.
+        -- inv Hsortedr. constructor; auto. constructor; auto.
+           ++ intros ? Hin; apply Hltr. constructor 2; auto.
+           ++ intros ? Hin; inv Hin; auto; try lia.
+              specialize (Hgtl _ H3); lia.
+        -- inv H6. constructor; auto. constructor; auto.
+           ++ intros ?; subst. contradiction H10; simpl.
+              constructor 1; rewrite find_ghost_set_equiv; constructor 2; constructor.
+           ++ rewrite -> empty_intersection in *.
+              intros ???; eapply H8; eauto.
+              constructor 1; rewrite find_ghost_set_equiv; constructor 1; auto.
+           ++ intros ?; contradiction H10; simpl.
+              constructor 1; rewrite find_ghost_set_equiv; constructor 1; auto.
+           ++ intros ?; rewrite -> empty_intersection in H8; eapply H8; eauto; simpl.
+              constructor 1; rewrite find_ghost_set_equiv; constructor 2; constructor.
+           ++ intros ?; subst. contradiction H11; simpl.
+              constructor 2; rewrite find_ghost_set_equiv; constructor 2; constructor.
+           ++ rewrite -> empty_intersection in *.
+              simpl; intros ? Hunion ?; inv Hunion.
+              rewrite find_ghost_set_equiv in H3; inv H3.
+              { eapply H8; eauto; simpl. constructor 2; rewrite find_ghost_set_equiv; constructor 1; auto. }
+              { inv H4; contradiction H10; simpl. constructor 2; rewrite find_ghost_set_equiv; constructor 1; auto. }
+              { rewrite find_ghost_set_equiv in H3; inv H3. eapply H19; eauto. inv H4; contradiction. }
+           ++ simpl; intros X; inv X.
+              { rewrite find_ghost_set_equiv in H0; inv H0; auto. inv H3; contradiction. }
+              { contradiction H11; simpl. constructor 1; auto. }
+           ++ intros ?; contradiction H11; simpl. constructor 2; rewrite find_ghost_set_equiv; constructor 1; auto.
+           ++ simpl; intros X; inv X.
+              { rewrite find_ghost_set_equiv in H0; inv H0; auto.
+                rewrite -> empty_intersection in H8; eapply H8; eauto; simpl. constructor 2; rewrite find_ghost_set_equiv; constructor 2; constructor.
+                inv H3. contradiction H10; simpl. constructor 2; rewrite find_ghost_set_equiv; constructor 2; constructor. }
+              { rewrite find_ghost_set_equiv in H0; inv H0; auto. inv H3; contradiction. }
+Qed.
+
+Lemma pushdown_tree_to_gmap : forall tg1 tg2,
+  (forall x y, In_ghost x tg1 -> In_ghost y tg2 -> Z.lt x y) ->
+  tree_to_gmap (pushdown_ghost tg1 tg2) = union (tree_to_gmap tg1) (tree_to_gmap tg2).
+Proof.
+  intros; revert dependent tg1; induction tg2; simpl; intros.
+  - rewrite right_id; auto.
+  - rewrite IHtg2_1.
+    rewrite -map_union_assoc insert_union_r; auto.
+    destruct (eq_dec (tree_to_gmap tg1 !! k) None); auto.
+    apply In_tree_to_gmap, (H _ k) in n; first lia.
+    constructor 1; auto.
+    { intros; apply H; auto.
+      constructor 2; auto. }
+Qed.
+
+Locate delete.
+Lemma delete_tree_to_gmap : forall tg x, sorted_ghost_tree tg ->
+  tree_to_gmap (delete_ghost x tg) = stdpp.base.delete x (tree_to_gmap tg).
+Proof.
+  intros; induction tg; auto; simpl.
+  - symmetry; apply delete_empty.
+  - inv H. destruct (Z.ltb x k) eqn: ?; [|destruct (Z.ltb k x) eqn: ?]; simpl.
+    + rewrite IHtg1; auto.
+      rewrite delete_insert_ne; last lia.
+      rewrite delete_union (delete_notin (tree_to_gmap tg2)); auto.
+      destruct (eq_dec (tree_to_gmap tg2 !! x) None); auto.
+      apply In_tree_to_gmap, Hltr in n; lia.
+    + rewrite IHtg2; auto.
+      rewrite delete_insert_ne; last lia.
+      rewrite delete_union (delete_notin (tree_to_gmap tg1)); auto.
+      destruct (eq_dec (tree_to_gmap tg1 !! x) None); auto.
+      apply In_tree_to_gmap, Hgtl in n; lia.
+    + rewrite pushdown_tree_to_gmap.
+      assert (x = k) by lia; subst; rewrite delete_insert; auto.
+      rewrite lookup_union.
+      destruct (eq_dec (tree_to_gmap tg1 !! k) None).
+      * rewrite e; destruct (eq_dec (tree_to_gmap tg2 !! k) None).
+        { rewrite e0; auto. }
+        apply In_tree_to_gmap, Hltr in n; lia.
+      * apply In_tree_to_gmap, Hgtl in n; lia.
+      * intros ?? ?%Hgtl ?%Hltr; lia.
+Qed.
+
+Lemma In_pushdown_left_ghost: forall (t1 t2: ghost_tree) (x: key),
+   In_ghost (V := val) x (pushdown_ghost t1 t2) -> In_ghost x t1 \/ In_ghost x t2.
+Proof.
+  intros. revert t2 H. induction t2; intros; simpl in *; auto. inv H.
+  - right. now apply InRoot_ghost.
+  - apply IHt2_1 in H1. destruct H1; [left | right]; auto. now apply InLeft_ghost.
+  - right. now apply InRight_ghost.
+Qed.
+
+Lemma pushdown_left_ghost_sorted: forall (tg1 tg2: ghost_tree),
+   sorted_ghost_tree tg1 -> sorted_ghost_tree tg2 -> 
+    (forall x y, In_ghost x tg1 -> In_ghost y tg2 -> Z.lt x y) ->
+   sorted_ghost_tree (V := val) (pushdown_ghost tg1 tg2).
+Proof.
+  intros. revert tg2 H0 H1. induction tg2; intros; simpl in H0 |-*; auto.
+  inv H0. constructor; auto.
+  - apply IHtg2_1; auto. intros. apply H1; auto. now apply InLeft_ghost.
+  - intros z ?. apply In_pushdown_left_ghost in H0. destruct H0.
+    + apply H1; auto. now apply InRoot_ghost.
+    + now specialize (Hgtl _ H0).
+Qed.
+
+Lemma In_delete_ghost: forall (x: key) (t: ghost_tree) (y: key), In_ghost (V := val) y (delete_ghost x t) -> In_ghost y t.
+Proof.
+  intros. revert t H. induction t; intros; simpl in *; auto. destruct (Z.ltb x k).
+  - inv H; try ((now apply InLeft_ghost) || (now apply InRoot_ghost) || (now apply InRight_ghost)).
+    apply IHt1 in H1. now apply InLeft_ghost.
+  - destruct (Z.ltb k x).
+    + inv H; try ((now apply InLeft_ghost) || (now apply InRoot_ghost) || (now apply InRight_ghost)).
+      apply IHt2 in H1. now apply InRight_ghost.
+    + apply In_pushdown_left_ghost in H. destruct H; [apply InLeft_ghost | apply InRight_ghost]; easy.
+Qed.
+
+Lemma delete_ghost_sorted: forall (x: key) (t: ghost_tree),
+   sorted_ghost_tree t -> sorted_ghost_tree (V := val) (delete_ghost x t).
+Proof.
+  intros. revert t H. induction t; intros; simpl; auto. inv H.
+  destruct (Z.ltb x k) eqn: ?; [|destruct (Z.ltb k x) eqn: ?].
+  - constructor; auto. intros ??%In_delete_ghost. now apply Hgtl.
+  - constructor; auto. intros ??%In_delete_ghost. now apply Hltr.
+  - apply pushdown_left_ghost_sorted; auto. intros.
+    apply Hgtl in H; apply Hltr in H0; lia.
+Qed.
+
+Lemma in_tree_del : forall g s g1,
+  in_tree g g1 * ghost_ref g s |-- (|==> ghost_ref g (Subtract s g1))%I.
+Proof.
+  intros. unfold in_tree at 1. Intros sh1. iIntros "H".
+  rewrite ghost_part_ref_join.
+  iMod (part_ref_update(P := set_PCM) _ _ _ _ (Subtract (Singleton g1) g1) (Subtract s g1) with "H") as "H".
+  { intros. repeat constructor.
+    - inversion 1; subst.
+      inv H. inv H3. specialize (H x). contradict H.
+      inv H1. split; auto.
+    - inv H. apply Extensionality_Ensembles.
+      split; unfold Included; intros.
+      { inv H. inv H1.
+        apply Union_introl. split; auto.
+        apply Union_intror; auto. }
+      { inv H. inv H1. congruence.
+        split; auto.
+        apply Union_intror; auto.
+        inv H0. specialize (H x). contradict H.
+        split; auto. }
+    - intros. subst. auto.      
+  }
+  fold (ghost_part_ref(P := set_PCM) sh1 (Subtract (Singleton g1) g1) (Subtract s g1) g).
+  rewrite <- ghost_part_ref_join.
+  iDestruct "H" as "[H $]". iDestruct "H" as "_".  auto.
+  Qed.
+
+
+Lemma update_ghost_ref_delete: forall g gl gr s g_in, finite s ->
+  (in_tree g g_in * ghost_ref g s * in_tree g gr * in_tree g gl  |-- |==>
+    ghost_ref g (Subtract (Subtract s gl) gr) * in_tree g g_in)%I .
+Proof.
+  intros. iIntros "H". iDestruct "H" as "((Ha & Hc) & Hd)".
+  iDestruct "Ha" as "(Ha & Hb)".
+  iPoseProof (in_tree_del with "[$Hd $Hb]") as ">Hb".
+  iPoseProof (in_tree_del with "[$Hc $Hb]") as ">Hb".
+  iModIntro; iFrame.
+Qed.
+
+Lemma pushdown_find_ghost : forall t1 t2,
+  sorted_ghost_tree t1 -> sorted_ghost_tree t2 ->
+  find_ghost_set' (pushdown_ghost t1 t2) = Union (find_ghost_set' t1) (find_ghost_set' t2).
+Proof.
+  intros. revert dependent t1; induction t2; simpl; intros.
+  + now rewrite -> invariants.Union_comm, invariants.Union_Empty.
+  + inv H0. rewrite find_ghost_set_equiv.
+    rewrite IHt2_1; auto. rewrite (find_ghost_set_equiv t2_1).
+    unfold Add.
+    rewrite <- (invariants.Union_assoc (find_ghost_set' t1) _ (find_ghost_set t2_2 g0)).
+    rewrite -> (invariants.Union_assoc (find_ghost_set' t1) _ _). reflexivity.
+Qed.
+
+Lemma pushdown_left_ghost_unique: forall tg1 tg2,
+  sorted_ghost_tree tg1 -> sorted_ghost_tree tg2 ->
+  unique_gname tg1 -> unique_gname tg2 ->
+  Intersection (find_ghost_set' tg1) (find_ghost_set' tg2) = @Empty_set gname ->
+  (forall x y, In_ghost x tg1 -> In_ghost y tg2 -> Z.lt x y) ->
+  unique_gname (pushdown_ghost tg1 tg2).
+Proof.
+  induction tg2; simpl; intros; auto.
+  inv H0. inv H2. apply Unique_Tree; auto.
+  - apply IHtg2_1; auto.
+    rewrite -> empty_intersection in *; intros ???.
+    eapply H3; eauto.
+    constructor 1. rewrite find_ghost_set_equiv; constructor 1; auto.
+    { intros; apply H4; auto. apply InLeft_ghost; auto. }
+  - rewrite pushdown_find_ghost; auto.
+    rewrite -> empty_intersection in *; intros ? Hin ?.
+    inv Hin.
+    + eapply H3; eauto.
+      constructor 2. rewrite find_ghost_set_equiv; constructor 1; auto.
+    + eapply H13; eauto.
+  - rewrite pushdown_find_ghost; auto.
+    intros Hcontra; inv Hcontra; try contradiction.
+    rewrite -> empty_intersection in H3; eapply H3; eauto.
+    constructor 1; rewrite find_ghost_set_equiv; constructor 2; constructor.
+  - rewrite pushdown_find_ghost; auto.
+    intros Hcontra; inv Hcontra; try contradiction.
+    rewrite -> empty_intersection in H3; eapply H3; eauto.
+    constructor 2; rewrite find_ghost_set_equiv; constructor 2; constructor.
+Qed.
+
+Lemma delete_find_ghost_weak: forall x tg k,
+  sorted_ghost_tree tg -> In_ghost x tg ->
+  Ensembles.In (find_ghost_set' (delete_ghost x tg)) k ->
+  Ensembles.In (find_ghost_set' tg) k.
+Proof.
+  induction tg; simpl; intros.
+  - inv H1.
+  - inv H. inv H0; simpl in *.
+    + rewrite Z.ltb_irrefl in H1.
+      rewrite pushdown_find_ghost in H1; auto.
+      rewrite -> !find_ghost_set_equiv. inv H1; [constructor 1 | constructor 2]; constructor 1; auto.
+    + specialize (Hgtl _ H2). destruct (Z.ltb x k) eqn:?; try lia.
+      inv H1.
+      * rewrite -> !find_ghost_set_equiv in * |-*. (* H |-* does not rewrite the 2nd instance on goal *)
+      inv H.
+      apply Union_introl, Union_introl. apply IHtg1; auto.
+      { inv H0; constructor 1; constructor 2; constructor. }
+      * constructor 2; auto.
+    + specialize (Hltr _ H2). destruct (Z.ltb x k) eqn:?; try lia. 
+      destruct (Z.ltb k  x) eqn:?; try lia.
+      inv H1.
+      * constructor 1; auto.
+      * rewrite -> !find_ghost_set_equiv in * |-*. (* H |-* does not rewrite the 2nd instance on goal *)
+      inv H.
+      apply Union_intror, Union_introl. apply IHtg2; auto.
+      { inv H0; constructor 2; constructor 2; constructor. }
+Qed.
+
+Lemma delete_ghost_unique: forall x tg,
+  In_ghost x tg -> sorted_ghost_tree tg ->
+  unique_gname tg -> unique_gname (delete_ghost x tg).
+Proof.
+  induction tg; simpl; auto; intros.
+  inv H0; inv H1. inv H.
+  - rewrite Z.ltb_irrefl. apply pushdown_left_ghost_unique; auto.
+    intros. apply Hgtl in H. apply Hltr in H0. lia.
+  - specialize (Hgtl _ H1); destruct (Z.ltb x k) eqn:?; try lia. apply Unique_Tree; auto.
+    + rewrite -> empty_intersection in *; intros ???.
+      eapply H10; eauto.
+      apply delete_find_ghost_weak in H; auto.
+    + intros ?%delete_find_ghost_weak; auto.
+    + intros ?%delete_find_ghost_weak; auto.
+  - specialize (Hltr _ H1); destruct (Z.ltb x k) eqn:?; try lia. 
+    destruct (Z.ltb k x) eqn:?; try lia. apply Unique_Tree; auto.
+    + rewrite -> empty_intersection in *; intros ???.
+      eapply H10; eauto.
+      apply delete_find_ghost_weak in H0; auto.
+    + intros ?%delete_find_ghost_weak; auto.
+    + intros ?%delete_find_ghost_weak; auto.
+Qed.
+
+Lemma ghost_tree_pushdown_left: forall t g g_root g_in gl gr x v,
+  tree_rep g g_root t * in_tree g g_in * in_tree g gr |--
+  EX n, EX n0, EX o1:option ghost_info,
+  public_half g_in (n, n0, Some o1) *
+  (!!(o1 = Some (x,v,gl,gr)) -->
+     EX o3 : option ghost_info,
+     public_half gr (Finite_Integer x, n0, Some o3) *
+  ((in_tree g gl -* EX o2 : option ghost_info, (public_half gl (n, Finite_Integer x, Some o2) * ((
+      (!!(o1 = Some (x,v,gl,gr) /\ o3 = None /\ (key_in_range x (n,n0) = true)) &&
+      public_half g_in (n, n0, Some o2) -* |==> tree_rep g g_root (base.delete x t) * in_tree g g_in)))))%I
+    && ((* turn_left *)(ALL gr1 gr2 : gname, ALL k : key, ALL y : val,
+        (!!(o1 = Some (x,v,gl,gr) /\ o3 = Some (k, y, gr1, gr2)
+          /\ (key_in_range x (n,n0) = true /\ less_than (Finite_Integer x) (Finite_Integer k) = true)) &&
+        (public_half g_in (n, n0, Some (Some (k, y, gr, gr2)))
+        * public_half gr (n, Finite_Integer k, Some (Some (x, v, gl, gr1))))
+        -* |==> tree_rep g g_root t * in_tree g g_in * in_tree g gr)))%I)).
+Proof.
+  intros. unfold tree_rep at 1. Intros tg.
+  sep_apply node_exist_in_tree; Intros.
+  sep_apply (ghost_tree_delete tg g_root g_in gl gr x v); auto.
+  Intros n n0 o1; Exists n n0 o1; cancel.
+  apply imp_andp_adjoint; Intros; subst.
+  rewrite prop_imp; [|auto].
+  Intros o3; Exists o3; cancel.
+  iIntros "(((Hcase & Hin) & Href) & Hr)"; iSplit.
+  + iDestruct "Hcase" as "[Hcase _]"; iDestruct "Hcase" as (o2) "(Hx & Hcase)".
+    iIntros "Hl"; iExists o2. iFrame "Hx".
+    iIntros "[(% & % & %) Hpub]"; subst.
+    iPoseProof (update_ghost_ref_delete with "[$Hin $Href $Hr $Hl]") as "Href".
+    { apply find_ghost_set_finite. }
+    repeat logic_to_iris. iMod "Href" as "[? $]".
+    iMod ("Hcase" with "[$Hpub]") as "[(% & % & % & %) ?]"; [auto|].
+    iModIntro.
+    unfold tree_rep. iExists (delete_ghost x tg).
+    rewrite H7 delete_tree_to_gmap; auto; iFrame.
+    iPureIntro; split; auto; split3.
+    * intros ?%delete_find_ghost_weak; auto.
+    * apply delete_ghost_unique; auto.
+    * split; auto; apply delete_ghost_sorted; auto.
+  + iDestruct "Hcase" as "[_ Hcase]".
+    iIntros (gr1 gr2 k y) "H".
+    iSpecialize ("Hcase" $! gr1 gr2 k y with "H").
+    repeat logic_to_iris. iMod "Hcase" as (tg') "[(% & % & % & %) ?]"; iModIntro.
+    unfold tree_rep; iFrame.
+    iExists tg'.
+    rewrite -> !find_ghost_set_equiv, !H5 in *; iFrame; auto.
+Qed.
+
+Lemma public_update : forall g (a b a' : G), my_half g gsh1 a * public_half g b |-- 
+  (|==> my_half g gsh1 a' * public_half g a')%I.
+Proof.
+  intros; unfold public_half'.
+  assert_PROP (sepalg.joins a (b.1, None)).
+  { iIntros "(my1 & my2 & ?)".
+    iPoseProof (own_valid_2(RA := ref_PCM _) with "[$my1 $my2]") as "%"; iPureIntro.
+    destruct H as ((?, ?) & [J ?] & ?); simpl in *.
+    destruct g0 as [(?, ?)|]; try contradiction.
+    eexists; apply J. }
+  destruct H.
+  erewrite <- sepcon_assoc, my_half_join by eauto.
+  sep_apply (public_update g x b a'); Intros; subst x.
+  erewrite <- my_half_join with (a1 := a')(a2 := (fst a', None)); eauto.
+  rewrite sepcon_assoc; apply derives_refl.
+  { split; hnf; simpl.
+    * symmetry; apply merge_id.
+    * constructor.
+  }
+Qed.
+
+
+
